fibo with refinements, pruning SMT context

pulse/share/steel/examples/pulse/Fibonacci.fst
@@ -47,3 +47,37 @@ fn fibo (n:pos)
   r
 }
 ```
+
+```pulse
+fn fibo2 (n:pos)
+  requires emp
+  returns r:nat
+  ensures pure (r == fib n)
+{
+  let mut i = ( 1 <: nat );
+  let mut j = ( 1 <: nat );
+  let mut ctr = ( 1 <: pos );
+  while (let vctr = !ctr; (vctr < n))
+  invariant b . exists vi vj vctr. (
+     pts_to i full_perm vi `star`
+     pts_to j full_perm vj `star`
+     pts_to ctr full_perm vctr `star`     
+     pure (1 <= vctr /\
+           vctr <= n /\
+           vi == fib (vctr - 1) /\
+           vj == fib vctr /\
+           b == (vctr < n))
+  )
+  {
+     let vc = !ctr;
+     let vi = !i;
+     let vj = !j;
+     i := vj;
+     j := vi + vj;
+     ctr := vc + 1;
+     ()
+  };
+  let r = !j;
+  ( r <: nat )
+}
+```
